viper-total-heaps/TotalConsistencyInst.thy
@@ -5,6 +5,7 @@ begin
 
 subsection \<open>Internal Consistency Wellfoundness\<close>
 
+
 lemma mono_prop_downward_ord_consistent_internal_total_full:
   shows "mono_prop_downward_ord consistent_internal_total_full"
   unfolding mono_prop_downward_ord_def
@@ -20,25 +21,92 @@ proof standard+
 qed
 
 
+lemma rm_from_lpm_preserved_intcons:
+  assumes ctxt_wf: "ctxt_pred_syn_wf ctxt"
+      and extcons: "consistent_external ctxt (get_total_full \<omega>)"
+      and "p \<le> get_mp_total_full \<omega> lp"
+    shows "consistent_external ctxt (get_total_full (rm_from_lpm_total_full \<omega> lp p))"
+  apply standard
+  apply (rename_tac pid vs q nm')
+  apply (case_tac "(pid,vs) = lp")
+   defer
+  using extcons[unfolded consistent_external.simps]
+   apply simp
+proof -
+  fix pid vs q' nm'
+  assume lpm': "Some (q',nm') = get_fnm_total (get_total_full (rm_from_lpm_total_full \<omega> lp p)) (pid,vs)"
+     and "(pid, vs) = lp"
+  then obtain q nm where lpm: "Some (q,nm) = get_fnm_total (get_total_full \<omega>) (pid,vs)"
+    apply simp
+    by (metis (no_types, opaque_lifting) lpm' get_fnm_total.simps get_fnm_total_full.simps rm_from_lpm_total_full_inverse)
+  hence extcons_ploc: "consistent_external_wrt_ploc ctxt (get_total_full \<omega>\<lparr> get_nm_total := nm \<rparr>) (pid,vs) (Rep_posreal q)"
+    using extcons[unfolded consistent_external.simps]
+    by auto
+  show "consistent_external_wrt_ploc ctxt
+          (get_total_full (rm_from_lpm_total_full \<omega> lp p)\<lparr>get_nm_total := nm'\<rparr>) (pid,vs) (Rep_posreal q')"
+  proof (cases "p \<ge> Rep_posreal q")
+    case True
+    hence "get_fnm_total (get_total_full (rm_from_lpm_total_full \<omega> lp p)) (pid,vs) = None"
+      apply (cases "get_fnm_total_full \<omega> lp"; simp)
+      using \<open>(pid, vs) = lp\<close> lpm
+      by fastforce+
+    then show ?thesis
+      using lpm'
+      by auto
+  next
+    case False
+    have "nm' = (1 - p / Rep_posreal q) *\<^sub>s nm"
+      using lpm lpm'
+      apply (cases "get_fnm_total_full \<omega> lp"; simp)
+       apply (simp add: \<open>(pid, vs) = lp\<close>)
+      by (metis Some_Some_ifD \<open>(pid, vs) = lp\<close> fstI option.inject sndI)
+    have "q' = Abs_posreal (Rep_posreal q - p)"
+      using lpm lpm'
+      apply (cases "get_fnm_total_full \<omega> lp"; simp)
+       apply (simp add: \<open>(pid, vs) = lp\<close>)
+      by (metis Some_Some_ifD \<open>(pid, vs) = lp\<close> fstI option.inject sndI)
+    have "(1 - p / Rep_posreal q) * Rep_posreal q = Rep_posreal q - p / Rep_posreal q * Rep_posreal q"
+      using False
+      apply (simp add: preal_to_real)
+      by (metis comm_monoid_mult_class.mult_1 divide_le_eq_1_pos eq_divide_eq left_diff_distrib less_eq_real_def linorder_le_cases prat_non_negative)
+    hence *: "(1 - p / Rep_posreal q) * Rep_posreal q =
+             Rep_posreal (Abs_posreal (Rep_posreal q - p))"
+      apply (simp add: preal_to_real)
+      using False PosReal.ppos.rep_eq gr_0_is_ppos less_eq_preal.rep_eq minus_preal.rep_eq posreal_to_preal(8) prat_non_negative
+      by auto
+
+    show ?thesis
+      using fraction_consistent_external(1)[OF ctxt_wf extcons_ploc, of "1 - p / Rep_posreal q"]
+      apply simp
+      unfolding \<open>nm' = _\<close> \<open>q' = _\<close>
+      using *
+      by fastforce
+  qed
+qed
+
+
 lemma wf_total_consistency_internal:
   assumes "ctxt_pred_syn_wf ctxt"
       and "ctxt_pred_self_framing_sat ctxt consistent_internal_total"
     shows "wf_total_consistency ctxt consistent_internal_total_full consistent_internal_total"
   unfolding wf_total_consistency_def
   apply (intro conjI)
-           apply (rule intcons_total_full_mono_prop_downward)
-          apply (simp add: intcons_empty is_empty_total_full_def)
+             apply (rule intcons_total_full_mono_prop_downward)
+            apply (simp add: intcons_empty is_empty_total_full_def)
   using intcons_preserved_by_red_stmt
-         apply blast
-        apply (simp add: intcons_preserved_by_update_store)
+           apply blast
+          apply (simp add: intcons_preserved_by_update_store)
   using consistent_internal_total_full_def
-       apply blast
+         apply blast
   using extcons_preserved_by_red_stmt
-      apply blast
+        apply blast
   subgoal
     unfolding consistent_internal_total_def consistent_internal_def wf_mask_simple_def
     by (metis get_mh_total.simps mh_le_nm_loc_sum order_trans)
   using unfold_preserves_internal_consistency_total
+      apply blast
+     apply (metis mono_prop_downward_ord_consistent_internal_total_full mono_prop_downward_ord_def rm_from_lpm_total_full_smaller)
+  using assms(1) rm_from_lpm_preserved_intcons
     apply blast
   by fact+
 
